Fp/Packing.lean
@@ -27,6 +27,7 @@ def PackedFloat.unpack (pf : PackedFloat e s)
 @[bv_normalize]
 def EUnpackedFloat.pack (uf : EUnpackedFloat (exponentWidth e s) (s + 1))
   : PackedFloat e s :=
+  -- min normal <= exp
   let inNormalRange := (BitVec.ofInt _ (minNormalExp e)).sle uf.exp
   {
     sign := uf.sign
@@ -42,11 +43,35 @@ def EUnpackedFloat.pack (uf : EUnpackedFloat (exponentWidth e s) (s + 1))
            else bif uf.isInfinite || uf.isZero then
             (0#_)
            else bif inNormalRange then
-            uf.sig.truncate _
+            uf.sig.truncate s -- drop the leading 1 bit
            else -- bif uf.isSubnorm then
+            -- shift right by #of subnormal bits.
             let shift := BitVec.ofInt _ (minNormalExp e) - uf.exp
-            (uf.sig >>> shift).truncate _
+            -- shift, and then truncate to significand width.
+            (uf.sig >>> shift).truncate s
+
   }
+
+
+namespace PackingExpAdjust
+def startUnpacked := (EUnpackedFloat.mkNumber { sign := true, ex := 0x2f#6, sig := 0x6#3 : UnpackedFloat _ _ })
+def expectedPacked : PackedFloat 5 2 := { sign := true, ex := 0x00#5, sig := 0x1#2 }
+
+/-- info: some (-3 / 262144) -/
+#guard_msgs in #eval startUnpacked.toRat?
+
+/-- info: some (-1 / 65536) -/
+#guard_msgs in #eval expectedPacked.toRat?
+
+
+-- theorem qeq : startUnpacked.toRat? = expectedPacked.toRat? := rfl
+
+end PackingExpAdjust
+
+-- This packs and just returns 0,
+/-- info: { sign := -, ex := 0x00#5, sig := 0x0#2 } -/
+#guard_msgs in #eval
+  (EUnpackedFloat.mkNumber { sign := true, ex := 0x2f#6, sig := 0x6#3 : UnpackedFloat _ _ }).pack (e := 5) (s := 2)
 
 theorem PackedFloat.isInfinite_pack_unpack (pf : PackedFloat 5 10) (hpf : pf.unpack.isInfinite) :
     pf.unpack.pack.isInfinite = pf.isInfinite ∧ pf.unpack.pack.sign = pf.sign := by
@@ -59,6 +84,7 @@ theorem PackedFloat.isNaN_pack_unpack (pf : PackedFloat 5 10) :
 theorem PackedFloat.pack_unpack (pf : PackedFloat 5 10) (hpf : pf.isNormOrSubnorm) :
     pf.unpack.pack = pf := by
   bv_decide
+
 
 /-- info: { sign := +, ex := 0x00#5, sig := 0x001#10 } -/
 #guard_msgs in #eval { sign := false, ex := 0x00#5, sig := 0x001#10 : PackedFloat _ _ }.unpack.pack
