Fp/UnpackedRound.lean
@@ -1,0 +1,878 @@
+import Fp.Basic
+import Fp.Rounding
+import Fp.MulInv
+import Fp.Proofs.Grind
+import Fp.ForLean.Rat
+
+@[bv_normalize]
+def BitVec.leadingOne (w : Nat) : BitVec w :=
+  1#w <<< (w - 1)
+
+@[simp]
+def BitVec.getElem_leadingOne (w : Nat) (i : Nat) (hi : i < w ) : (BitVec.leadingOne w)[i] = decide (i = w - 1) := by
+  simp [leadingOne]
+  grind
+
+@[bv_normalize]
+def BitVec.decrement (x : BitVec w) : BitVec w := x - 1#w
+
+@[bv_normalize]
+def BitVec.extendAtMsb (x : BitVec w) (δ : Nat) : BitVec (δ + w) :=
+  x.zeroExtend _
+
+/-- Extract from the MSB, starting at msb lo, going downward for 'len' bits.
+0<----------------------->(w-1)
+----------->loMsb----|len
+           |
+            <-----------------loLsb
+
+-/
+@[bv_normalize]
+def BitVec.extractMsb' (x : BitVec w) (loMsb : Nat) (len : Nat) :
+    BitVec len :=
+  (x.reverse.extractLsb' loMsb len).reverse
+
+theorem BitVec.getLsbD_extractMsb' {w lo len : Nat} (x : BitVec w)
+    (i : Nat):
+    (extractMsb' x lo len).getMsbD i =
+    (x.getMsbD (lo + i) && decide (i < len) && decide (lo + i < w)) := by
+  simp [extractMsb', BitVec.getMsbD_eq_getLsbD, BitVec.getLsbD_reverse]
+  by_cases h1 : i < len
+  · simp [h1]
+    simp [show len - 1 - i < len by omega]
+    simp [show len - 1 - (len - 1 - i) < len by omega]
+    simp [show len - 1 - (len - 1 - i) = i by omega]
+    intros h2 h3
+    have := BitVec.lt_of_getLsbD h3
+    omega
+  · simp [h1]
+
+@[bv_normalize]
+def BitVec.expandingSubtract {w} (a b : BitVec w) : BitVec (w + 1) :=
+  let a' : BitVec (w + 1) := a.signExtend (w + 1)
+  let b' : BitVec (w + 1) := b.signExtend (w + 1)
+  a' - b'
+
+
+@[simp]
+theorem BitVec.toInt_expandingSubtract {w} (a b : BitVec w) :
+  (expandingSubtract a b).toInt = a.toInt - b.toInt := by
+  simp [expandingSubtract, toInt_signExtend]
+  have : 2 ^ (w + 1) / 2 = 2^w := by grind
+  apply Int.bmod_eq_of_le <;> grind
+
+
+@[bv_normalize]
+def BitVec.width {w : Nat} (_x : BitVec w) : Nat := w
+
+/-- bitvector that has 1 at index i and 0 everywhere else. -/
+@[bv_normalize]
+def BitVec.oneHotBV (i : BitVec w) : BitVec w :=
+    1#w <<< i
+
+@[simp]
+theorem BitVec.getlsbD_oneHotBV (i : BitVec w) :
+    (oneHotBV i).getLsbD j =
+    (decide (j < w) && decide (i.toNat = j)) := by
+  simp [oneHotBV]
+  by_cases h1 : j < w
+  · simp [h1]
+    grind
+  · simp [h1]
+
+@[simp]
+theorem BitVec.getElem_oneHotBV (i : BitVec w) (j : Fin w) :
+    (oneHotBV i)[j] = decide (i.toNat = j) := by
+  simp [← BitVec.getLsbD_eq_getElem]
+
+/-- Convert a binary number into a unary mask of that number. -/
+@[bv_normalize]
+def BitVec.orderEncode (x : BitVec w) : BitVec w :=
+  (oneHotBV x) - 1
+
+theorem BitVec.orderEncode_eq_oneHotBV_sub (x : BitVec w) :
+    BitVec.orderEncode x = oneHotBV x - 1 := rfl
+
+@[simp]
+theorem BitVec.orderEncode_eq_allOnes_of_le {w : Nat} (x : BitVec w)
+    (h : w ≤ x.toNat) :
+    orderEncode x = allOnes w := by
+  simp [orderEncode, oneHotBV]
+  rw [BitVec.shiftLeft_eq_zero]
+  · simp [BitVec.neg_one_eq_allOnes]
+  · omega
+
+axiom AxOrderEncode {P : Prop} : P
+
+theorem BitVec.getLsbD_orderEncode_of_lt (x : BitVec w) (i : Nat) (hi : i < w) :
+    (orderEncode x).getLsbD i = (decide (i < x.toNat)) := by
+  by_cases hi : x.toNat < w
+  · rw [orderEncode]
+    · -- ⊢ (1#w <<< x - 1).getLsbD i = decide (i < x.toNat)
+      exact AxOrderEncode
+  · rw [BitVec.orderEncode_eq_allOnes_of_le]
+    · simp; omega
+    · omega
+
+theorem BitVec.getElem_orderEncode_of_lt {w : Nat} (x : BitVec w) (i : Nat) (hi : i < w) :
+    (orderEncode x)[i] = (decide (i < x.toNat)) := by
+  rw [← getLsbD_eq_getElem]
+  apply BitVec.getLsbD_orderEncode_of_lt x i hi
+
+@[simp]
+theorem BitVec.getLsbD_orderEncode {w : Nat} (x : BitVec w) (i : Nat) :
+    (orderEncode x).getLsbD i = (decide (i < x.toNat) && decide (i < w)) := by
+  by_cases hi : i < w
+  · simp [hi]
+    rw [BitVec.getElem_orderEncode_of_lt]
+  · rw [BitVec.getLsbD_of_ge x.orderEncode i (by omega)]
+    simp; omega
+
+@[simp]
+theorem BitVec.getElem_orderEncode {w : Nat} (x : BitVec w) (i : Nat) (hi : i < w) :
+    (orderEncode x)[i] = (decide (i < x.toNat)) := by
+  rw [← getLsbD_eq_getElem]
+  rw [BitVec.getLsbD_orderEncode x i]
+  simp [hi]
+
+@[simp]
+theorem BitVec.orderEncode_eq_shiftRight_allOnes {x : BitVec w} :
+    orderEncode x = BitVec.allOnes w >>> (w - x.toNat) := by
+  ext i hi
+  simp
+  omega
+
+@[bv_normalize]
+def BitVec.scollar (x : BitVec w) (minVal : BitVec w) (maxVal : BitVec w) : BitVec w :=
+  if x.slt minVal then minVal
+  else if maxVal.slt x then maxVal
+  else x
+
+-- roundingDecision mode inUf.sign significandEven choosenGuardBit choosenStickyBit false
+-- bollu: TODO: port rounding mode for real.
+@[bv_normalize]
+def roundingDecision (mode : RoundingMode) (sign : Bool) (significandEven : Bool)
+  (guardBit : Bool) (stickyBit : Bool) (exact : Bool) : Bool :=
+  match mode with
+  | RoundingMode.RNE =>
+      (guardBit && (stickyBit || !significandEven))
+  | _ => false
+
+@[bv_normalize]
+def rounderSpecialCases
+  (roundingMode : RoundingMode)
+  (roundedResult : UnpackedFloat (exponentWidth targetExponentWidth targetSignificandWidth) (targetSignificandWidth + 1))
+  (overflow : Bool)
+  (underflow : Bool)
+  (isZero : Bool) : EUnpackedFloat (exponentWidth targetExponentWidth targetSignificandWidth) (targetSignificandWidth + 1) :=
+  let returnInf : Bool :=
+    match roundingMode with
+    | RoundingMode.RNE => true
+    | RoundingMode.RNA => true
+    | RoundingMode.RTP => !roundedResult.sign
+    | RoundingMode.RTN => roundedResult.sign
+    | _ => false
+  let returnZero : Bool :=
+    match roundingMode with
+    | RoundingMode.RNE => true
+    | RoundingMode.RNA => true
+    | RoundingMode.RTZ => true
+    | RoundingMode.RTP => roundedResult.sign
+    | RoundingMode.RTN => !roundedResult.sign
+
+  let inf : EUnpackedFloat (exponentWidth targetExponentWidth targetSignificandWidth) (targetSignificandWidth + 1) :=
+    EUnpackedFloat.mkInfinity roundedResult.sign
+  let max : EUnpackedFloat (exponentWidth targetExponentWidth targetSignificandWidth) (targetSignificandWidth + 1) :=
+    EUnpackedFloat.mkNumber <|
+    { sign := roundedResult.sign,
+      ex := BitVec.ofInt (exponentWidth targetExponentWidth targetSignificandWidth) (maxNormalExp targetExponentWidth),
+      sig := BitVec.allOnes (targetSignificandWidth + 1) }
+  let min : EUnpackedFloat (exponentWidth targetExponentWidth targetSignificandWidth) (targetSignificandWidth + 1) :=
+    EUnpackedFloat.mkNumber <|
+    { sign := roundedResult.sign,
+      ex := BitVec.ofInt (exponentWidth targetExponentWidth targetSignificandWidth) (minSubnormalExp targetExponentWidth targetSignificandWidth),
+      sig := BitVec.leadingOne (targetSignificandWidth + 1) }
+  let zero : EUnpackedFloat (exponentWidth targetExponentWidth targetSignificandWidth) (targetSignificandWidth + 1) :=
+    EUnpackedFloat.mkZero roundedResult.sign
+
+  if isZero then
+    zero
+  else if underflow then
+    if returnZero then
+      zero
+    else
+      min
+  else if overflow then
+    if returnInf then
+      inf
+    else
+      max
+  else
+    EUnpackedFloat.mkNumber <| roundedResult
+
+axiom AxRoundPreconditions {P : Prop} : P
+
+def mkPackedFloats (E : Nat) (S : Nat) : Array (PackedFloat E S) := Id.run do
+  let mut res := #[]
+  for expVal in [0:Nat.pow 2 E] do
+    for sigVal in [0:Nat.pow 2 S] do
+      for sign in [true, false] do
+        let pf : PackedFloat E S :=
+          { sign := sign,
+            ex := BitVec.ofNat E expVal,
+            sig := BitVec.ofNat S sigVal }
+        res := res.push pf
+  res
+
+/--
+Return all representable packed floats of given exponent and significand widths,
+in ascending order by their rational value.
+-/
+def mkPackedFloatNumsSorted (E : Nat) (S : Nat) :
+    Array (PackedFloat E S × Rat) := Id.run do
+  let pfs ← mkPackedFloats E S
+  let mut res := #[]
+  for pf in pfs do
+    if let .some r := pf.toRat? then
+      res := res.push (pf, r)
+  res.qsort (fun a b => a.2 < b.2)
+
+/-
+Implementation of RNE rounding by finding the closest representable float, exhaustively.
+Note that zero needs special handling, because toRat does not distinguish +0 and -0,
+but FP does.
+-/
+def getClosestRNEResult {expWidth sigWidth : Nat}
+    (targetExponentWidth targetSignificandWidth : Nat)
+    (inUf : UnpackedFloat expWidth sigWidth) :
+    EUnpackedFloat (exponentWidth targetExponentWidth targetSignificandWidth) (targetSignificandWidth + 1) := Id.run do
+  let inRat := inUf.toRat
+  let candidates := mkPackedFloatNumsSorted targetExponentWidth targetSignificandWidth
+  if inRat < (candidates.getD 0 default).2 then
+    EUnpackedFloat.mkInfinity true
+  else if inRat > (candidates.getD (candidates.size - 1) default).2 then
+    EUnpackedFloat.mkInfinity false
+  else
+    let candidatesWithDist := candidates.map (fun (pf, r) =>
+      (pf, r, (inRat - r).abs))
+    let candidatesSorted := candidatesWithDist.qsort (fun a b => a.2.2 < b.2.2)
+    let out1 := candidatesSorted.getD 0 default
+    let out2 := candidatesSorted.getD 1 default
+    let (pf1, r1, dist1) := out1
+    let (pf2, _r2, dist2) := out2
+    if r1 = 0 then
+      EUnpackedFloat.mkZero inUf.sign
+    else
+      if hlt : dist1 < dist2 then
+        pf1.unpack
+      else if hgt : dist2 < dist1 then
+        pf2.unpack
+      else
+        have : dist1 = dist2 := by grind
+          -- round to the nearest even number
+          if r1.num % 2 == 0 then
+            pf1.unpack
+          else
+            pf2.unpack
+          -- round to nearest even.
+
+def BitVec.toBitsStr {w : Nat} (bv : BitVec w) : String := Id.run do
+  let mut s := "0b"
+  for i in [0:w] do
+    let bit := if bv.getMsbD i then "1" else "0"
+    s := s.append bit
+  s
+
+@[bv_normalize]
+def BitVec.isZero {w : Nat} (bv : BitVec w) : Bool :=
+  bv = BitVec.ofNat w 0
+
+/-- conditionally increment, and return flag of whether overflow was observed -/
+@[bv_normalize]
+def conditionalIncrementWithFlags (cond : Bool) (x : BitVec w) : BitVec w × Bool :=
+  if cond then
+    let x' := x.zeroExtend (w + 1) + 1#(w + 1)
+    (x'.setWidth w, x'.msb)
+  else
+    (x, false)
+
+def BitVec.smin (a b : BitVec w) : BitVec w :=
+  if a.slt b then a else b
+
+def BitVec.smax (a b : BitVec w) : BitVec w :=
+  -- a > b then a else b
+  -- b < a
+  if b.slt a then a else b
+
+
+/-- A variant of 'getLsbD' where the index is also a bitvector. -/
+@[bv_normalize]
+def BitVec.getLsbDBV {w : Nat} (x : BitVec w) (i : BitVec w) : Bool :=
+  x &&& (1#w <<< i) ≠ 0#w
+
+example (x y : BitVec 5) (hy : y < 3#5) : (x <<< 3#5).getLsbDBV y = false := by
+  bv_decide
+
+@[simp]
+theorem BitVec.getLsbDBV_eq_getLsbD {w : Nat} (x : BitVec w) (i : BitVec w) :
+    x.getLsbDBV i = x.getLsbD (i.toNat) := by
+  rw [getLsbDBV]
+  simp
+  by_cases hx : x &&& (1#w <<< i.toNat) = 0#w
+  · rw [hx]
+    simp
+    have : (x &&& (1#w <<< i.toNat)).getLsbD i.toNat = false := by
+      grind
+    grind
+  · simp [hx]
+    simp at hx
+    have : (x &&& (1#w <<< i.toNat)).getLsbD i.toNat = true := by
+      simp
+      grind
+    grind
+
+def BitVec.getMsbDBV {w : Nat} (x : BitVec w) (i : BitVec w) : Bool :=
+  x.getLsbDBV ((BitVec.ofNat w (w - 1)) - i)
+
+@[simp]
+theorem BitVec.getMsbDBV_eq_getMsbD {w : Nat} (x : BitVec w) (i : BitVec w)
+    (hi : i.toNat < w) :
+    x.getMsbDBV i = x.getMsbD (i.toNat) := by
+  have : w - 1 < 2^w := by
+    have : w < 2^w := by exact Nat.lt_two_pow_self
+    grind
+  rw [getMsbDBV, getLsbDBV_eq_getLsbD]
+  rw [BitVec.toNat_sub_of_le]
+  · simp
+    rw [Nat.mod_eq_of_lt (by omega)]
+    simp [BitVec.getMsbD]
+    omega
+  · rw [BitVec.le_def]
+    simp only [toNat_ofNat]
+    rw [Nat.mod_eq_of_lt (by omega)]
+    omega
+
+/--
+Extract the bits from LSB from low index `0` to high index `start` (excluded), setting other bits to zero.
+-/
+def BitVec.extractLsbTo0BV {w : Nat} (x : BitVec w) (start : BitVec w) : BitVec w :=
+  x &&& (orderEncode start)
+
+@[simp]
+theorem BitVec.getLsbD_extractLsbTo0BV_eq_decide {w : Nat} (x : BitVec w) (start : BitVec w) (i : Nat) :
+    (x.extractLsbTo0BV start).getLsbD i = (x.getLsbD i &&  decide (i < start.toNat)) := by
+  rw [extractLsbTo0BV]
+  rw [BitVec.getLsbD_and]
+  rw [BitVec.getLsbD_orderEncode]
+  by_cases hi : i < w
+  · by_cases hstart : start.toNat < w
+    · have : start.toNat < 2^w := by
+        have : w < 2^w := by exact Nat.lt_two_pow_self
+        omega
+      simp [hi]
+    · simp [hi]
+  · simp [hi]
+    intros hx
+    have := BitVec.lt_of_getLsbD hx
+    omega
+
+
+/--
+Extract out bits from 'startMsb' (excluded) down to low index `0`, setting other bits to zero.
+-/
+def BitVec.maskMsbTo0BV {w : Nat} (x : BitVec w) (startMsb : BitVec w) : BitVec w :=
+  BitVec.extractLsbTo0BV x (BitVec.ofNat w w  - startMsb)
+
+/--
+observe that the bounds are sane.
+if startMsb = 0, then we extract the full vector, and the decide is just (i < w).
+if startMsb = 1, then we extract all but the MSB, and the decide is (i < w - 1).
+if startMsb = w, then we extract nothing, and the decide is (i < 0) which is always false.
+-/
+@[simp]
+theorem BitVec.getMsbD_extractMsbTo0BV_eq_decide {w : Nat}
+    (x : BitVec w)
+    (startMsb : BitVec w)
+    (i : Nat)
+    (hstart : startMsb.toNat ≤ w) :
+    (x.maskMsbTo0BV startMsb).getLsbD i =
+      (x.getLsbD i &&  decide (i < (w - startMsb.toNat))) := by
+  rw [maskMsbTo0BV]
+  rw [BitVec.getLsbD_extractLsbTo0BV_eq_decide]
+  by_cases hx : x.getLsbD i
+  · simp only [hx, Bool.true_and, decide_eq_decide]
+    rw [BitVec.toNat_sub_of_le]
+    · simp
+    · rw [BitVec.le_def]
+      simp
+      omega
+  · simp [hx]
+
+
+/-- a > b -/
+@[bv_normalize]
+def BitVec.sgt {w : Nat} (a b : BitVec w) : Bool :=
+  b.slt a
+
+
+/--
+This implementation performs rounding, with many redundant checks
+to help with debugging.
+
+Preconditions for rounding to succeed:
+
+(hs : sigWidth >= targetSignificandWidth + 1 + 2)
+(he : expWidth >= targetExponentWidth)
+(hs' : sigWidth >= 1) :
+-/
+@[bv_normalize]
+def UnpackedFloat.debugRound {expWidth sigWidth : Nat} {targetExponentWidth targetSignificandWidth : Nat}
+  (inUf : UnpackedFloat expWidth sigWidth)
+  (mode : RoundingMode) :
+  (EUnpackedFloat (exponentWidth targetExponentWidth targetSignificandWidth) (targetSignificandWidth + 1) × String) :=
+  let out := ""
+  -- round a normalized, normal float.
+  let out := out ++ s!"\n--- rounding: {repr inUf} ---"
+  let out := out ++ s!"\n  val (Q): {inUf.toRat} = sig({inUf.sig.toBitsStr}=nat:{inUf.sig.toNat})) * 2 ** exp:([{inUf.ex.toBitsStr}=int:{inUf.ex.toInt}] - ({sigWidth - 1}))"
+  let exp : BitVec expWidth := inUf.ex
+
+  let targetMinNormalExp : BitVec expWidth :=
+    BitVec.ofInt expWidth (minNormalExp targetExponentWidth)
+  let out := out ++ s!"\nexp: {exp.toBitsStr} = int:{exp.toInt}"
+  let out := out ++ s!"\ntargetMinNormalExp: {targetMinNormalExp.toBitsStr} = int:{targetMinNormalExp.toInt}"
+  let out := if targetMinNormalExp.toInt != minNormalExp targetExponentWidth then
+    out ++ "\nERROR: targetMinNormalExp.toInt != minNormalExp targetExponentWidth"
+  else
+    out
+
+  let out := out ++ s!"\nmaxNormalExp: {maxNormalExp targetExponentWidth}"
+  let earlyOverflow : Bool := exp.sgt (BitVec.ofInt expWidth (maxNormalExp targetExponentWidth))
+  let out := out ++ s!"\nearlyOverflow: {earlyOverflow}"
+  let out := out ++ s!"\nminSubnormalExp: {minSubnormalExp targetExponentWidth targetSignificandWidth}"
+  let earlyUnderflow : Bool := exp.slt (BitVec.ofInt expWidth (minSubnormalExp targetExponentWidth targetSignificandWidth))
+  let out := out ++ s!"\nearlyUnderflow: {earlyUnderflow}"
+
+  -- force exponent to be at least min normal exponent.
+  let expGeMin :=
+    if exp.slt targetMinNormalExp then
+      targetMinNormalExp
+    else
+      exp
+  let out := out ++ s!"\nexpGeMin: {expGeMin.toBitsStr} = int:{expGeMin.toInt}"
+
+  -- how much to shift 'sig' by.
+  let shiftAmtPositive := expGeMin - exp
+  let out := out ++ s!"\nshiftAmtPositive: {shiftAmtPositive.toBitsStr} = int:{shiftAmtPositive.toInt} = nat:{shiftAmtPositive.toNat}"
+  -- have : shiftAmtPositive.toInt ≥ 0 := AxRoundNormal
+  -- have : shiftAmtPositive.toNat = shiftAmtPositive.toInt := AxRoundNormal
+  -- have : exp.toInt + shiftAmtPositive.toInt = expGeMin.toInt := AxRoundNormal
+
+  let sigWithHidden : BitVec sigWidth := inUf.sig
+  let out := out ++ s!"\nsigWithHidden: {sigWithHidden.toBitsStr} = nat:{sigWithHidden.toNat}"
+
+  -- in inf precision, we want to take:
+  --                ↓ guard
+  --  1 . a b c d e f g h ... * 2^exp
+  --  ============↑ (6 bits of precision)
+  -- suppose we exceed by 3 bits, so shiftAmt = 3.
+
+  -- and convert to target precision:
+  --                  ↓ guard
+  --  0 . 0 0 0 1 a b c d e f g h * 2^exp + 2^shiftAmt | to make 'exp + shiftAmt >= minNormalExp'.
+  --  ==============↑ (6 bits of precision)
+  -- (sigWidth - 1) - (targetSignificandWidth - 1) -
+  -- let targetSigWithHidden : BitVec (targetSignificandWidth + 1) :=
+  --   sigWithHidden.extractMsb' 0 (targetSignificandWidth + 1)
+  -- to grab the bit *after* w bits, it's the bit x[w].
+  -- we want the bit *after* targetSignificandWidth + 1, i.e., bit at index targetSignificandWidth + 1.
+  let out := out ++ s!"\nguardBitIndexFromLsb: (sigWidth({sigWidth}) - 1)  - (targetSignificandWidth({targetSignificandWidth}) + 1) = {(sigWidth - 1) - (targetSignificandWidth + 1)}"
+  let guardBitIndexFromLsb : BitVec sigWidth :=
+    BitVec.ofNat sigWidth ((sigWidth - 1) - (targetSignificandWidth + 1))
+  let out := out ++ s!"\nguardBitIndexFromLsb: {guardBitIndexFromLsb.toBitsStr} = nat:{guardBitIndexFromLsb.toNat}"
+  -- | See that when we call 'shiftAmtPositive.zeroExtend sigWidth', there is
+  -- a potential that shiftAmtPositive is wider than sigWidth.
+  -- However, when we compute early underflow,
+  let guardBitIndexFromLsbAdjusted : BitVec sigWidth :=
+    guardBitIndexFromLsb + shiftAmtPositive.zeroExtend sigWidth
+  let out := out ++ s!"\nguardBitIndexFromLsbAdjusted: {guardBitIndexFromLsbAdjusted.toBitsStr} = nat:{guardBitIndexFromLsbAdjusted.toNat}"
+
+  let guardBitMask : BitVec sigWidth := BitVec.oneHotBV guardBitIndexFromLsbAdjusted
+  let out := out ++ s!"\nguardBitMask: {guardBitMask.toBitsStr}"
+  let guardBit : Bool := (sigWithHidden &&& guardBitMask) ≠ 0#sigWidth
+  let out := out ++ s!"\nguardBit: {guardBit} = {sigWithHidden.toBitsStr} &&& {guardBitMask.toBitsStr}"
+  let stickyBitsMask : BitVec sigWidth := (BitVec.orderEncode guardBitIndexFromLsbAdjusted)
+  let out := out ++ s!"\nstickyBitsMask: {stickyBitsMask.toBitsStr}"
+  let stickyBits : BitVec sigWidth := (sigWithHidden &&& stickyBitsMask)
+  let out := out ++ s!"\nstickyBits: {stickyBits.toBitsStr}"
+  let stickyBit : Bool := stickyBits ≠ 0#sigWidth
+  let out := out ++ s!"\nstickyBit: {stickyBit} = {sigWithHidden.toBitsStr} &&& {stickyBitsMask.toBitsStr}"
+
+  let sigwithHiddenCleared : BitVec sigWidth :=
+    sigWithHidden &&& (~~~(guardBitMask ||| stickyBitsMask))
+  let out := out ++ s!"\nsigwithHiddenCleared: {sigwithHiddenCleared.toBitsStr} = {sigWithHidden.toBitsStr} &&& ~({guardBitMask.toBitsStr} ||| {stickyBitsMask.toBitsStr})"
+
+  let lsbMask : BitVec sigWidth :=
+     BitVec.oneHotBV (guardBitIndexFromLsbAdjusted + 1#sigWidth)
+  let out := out ++ s!"\nlsbMask: {lsbMask.toBitsStr}"
+
+  let isEven : Bool := sigWithHidden &&& lsbMask = 0#sigWidth
+  let out := out ++ s!"\nisEven: {isEven} = {sigWithHidden.toBitsStr} &&& {lsbMask.toBitsStr}"
+  let shouldRoundUp := roundingDecision
+    (mode := mode)
+    (sign := inUf.sign)
+    (significandEven := isEven)
+    (guardBit := guardBit)
+    (stickyBit := stickyBit)
+    (exact := false)
+  let out := out ++ s!"\nshouldRoundUp: {shouldRoundUp}"
+  let out := if shouldRoundUp then
+    out ++ s!"\nroundedTargetSigWithHidden = sigwithHiddenCleared({sigwithHiddenCleared.toBitsStr}) + lsbMask({lsbMask.toBitsStr})"
+  else
+    out ++ s!"\nroundedTargetSigWithHidden = sigwithHiddenCleared({sigwithHiddenCleared.toBitsStr})"
+  let sigDidOverflow_RoundedTargetSigWithHidden : BitVec (sigWidth + 1) :=
+    if shouldRoundUp then
+      sigwithHiddenCleared.zeroExtend (sigWidth + 1) + lsbMask.zeroExtend (sigWidth + 1)
+    else
+      sigwithHiddenCleared.zeroExtend (sigWidth + 1)
+
+  let sigDidOverflow : Bool :=
+    sigDidOverflow_RoundedTargetSigWithHidden.msb
+
+  let roundedTargetSigWithHidden : BitVec sigWidth :=
+    sigDidOverflow_RoundedTargetSigWithHidden.setWidth sigWidth
+
+  let out := out ++ s!"\nroundedTargetSigWithHidden: {roundedTargetSigWithHidden.toBitsStr} = nat:{roundedTargetSigWithHidden.toNat}"
+  let out := out ++ s!"\nsigDidOverflow: {sigDidOverflow}"
+
+  let roundedTargetSigWithHiddenOverflowAdjusted : BitVec sigWidth :=
+    if sigDidOverflow then
+      lsbMask
+    else
+      roundedTargetSigWithHidden
+  let out := out ++ s!"\nroundedTargetSigWithHiddenOverflowAdjusted: {roundedTargetSigWithHiddenOverflowAdjusted.toBitsStr} = nat:{roundedTargetSigWithHiddenOverflowAdjusted.toNat}"
+
+  let roundedExpDidOverflow_roundedExp : BitVec (expWidth + 1) :=
+    if sigDidOverflow then
+      exp.zeroExtend (expWidth + 1) + 1#(expWidth + 1)
+    else
+      exp.zeroExtend (expWidth + 1)
+
+  let roundedExpDidOverflow : Bool :=
+    roundedExpDidOverflow_roundedExp.msb
+
+  let roundedExp : BitVec expWidth :=
+    roundedExpDidOverflow_roundedExp.setWidth expWidth
+  let out := out ++ s!"\nroundedExp: {roundedExp.toBitsStr} = int:{roundedExp.toInt}"
+  let out := out ++ s!"\nroundedExpDidOverflow: {roundedExpDidOverflow}"
+  -- I find this width stuff confusing, which width should we use?
+  -- have : expWidth ≥ exponentWidth targetExponentWidth targetSignificandWidth := by grind
+  let maxNormalExpBV : BitVec (expWidth) :=
+    BitVec.ofInt (expWidth)
+      (maxNormalExp targetExponentWidth)
+  let lateOverflow : Bool :=
+    maxNormalExpBV.slt roundedExp
+  let out := out ++ s!"\nlate overflow: {lateOverflow} = roundedExp({roundedExp.toBitsStr}=int:{roundedExp.toInt}) > maxNormalExpBV({maxNormalExpBV.toBitsStr}=int:{maxNormalExpBV.toInt})"
+  let subnormalExpBV : BitVec (expWidth) :=
+    BitVec.ofInt (expWidth)
+      (subnormalExp targetExponentWidth)
+  let lateUnderflow : Bool :=
+    roundedExp.slt subnormalExpBV
+  let out := out ++ s!"\nlate underflow: {lateUnderflow} = maxNormalExpBV({maxNormalExpBV.toBitsStr}=int:{maxNormalExpBV.toInt}) < roundedExp({roundedExp.toBitsStr}=int:{roundedExp.toInt})"
+  let underflow : Bool := lateUnderflow || earlyUnderflow
+  let out := out ++ s!"\nunderflow: {underflow} = lateUnderflow({lateUnderflow}) || earlyUnderflow({earlyUnderflow})"
+  let overflow : Bool := lateOverflow || earlyOverflow || roundedExpDidOverflow
+  let out := out ++ s!"\noverflow: {overflow} = lateOverflow({lateOverflow}) || earlyOverflow({earlyOverflow})"
+
+  let finalExp := roundedExp.truncate (exponentWidth targetExponentWidth targetSignificandWidth)
+  let finalSigTruncated := roundedTargetSigWithHiddenOverflowAdjusted.extractMsb' 0 (targetSignificandWidth + 1)
+  let finalNumber : UnpackedFloat (exponentWidth targetExponentWidth targetSignificandWidth) (targetSignificandWidth + 1) :=
+    { sign := inUf.sign,
+      ex := finalExp,
+      sig := finalSigTruncated
+    }
+
+  let result := rounderSpecialCases
+    (roundingMode := mode)
+    finalNumber overflow underflow inUf.isZero
+  (result, out)
+
+/--
+The core rounding function, that rounds an `UnpackedFloat` to the target exponent and significand widths,
+-/
+@[bv_normalize]
+def UnpackedFloat.round {expWidth sigWidth : Nat} {targetExponentWidth targetSignificandWidth : Nat}
+  (inUf : UnpackedFloat expWidth sigWidth)
+  (mode : RoundingMode) :
+  EUnpackedFloat (exponentWidth targetExponentWidth targetSignificandWidth) (targetSignificandWidth + 1) :=
+  let exp : BitVec expWidth := inUf.ex
+  let targetMinNormalExp : BitVec expWidth :=
+    BitVec.ofInt expWidth (minNormalExp targetExponentWidth)
+  let earlyOverflow : Bool := exp.sgt (BitVec.ofInt expWidth (maxNormalExp targetExponentWidth))
+  let earlyUnderflow : Bool := exp.slt (BitVec.ofInt expWidth (minSubnormalExp targetExponentWidth targetSignificandWidth))
+  let expGeMin :=
+    if exp.slt targetMinNormalExp then
+      targetMinNormalExp
+    else
+      exp
+
+  -- how much to shift 'sig' by.
+  let shiftAmtPositive := expGeMin - exp
+  -- have : shiftAmtPositive.toInt ≥ 0 := AxRoundNormal
+  -- have : shiftAmtPositive.toNat = shiftAmtPositive.toInt := AxRoundNormal
+  -- have : exp.toInt + shiftAmtPositive.toInt = expGeMin.toInt := AxRoundNormal
+
+  let sigWithHidden : BitVec sigWidth := inUf.sig
+
+  -- in inf precision, we want to take:
+  --                ↓ guard
+  --  1 . a b c d e f g h ... * 2^exp
+  --  ============↑ (6 bits of precision)
+  -- suppose we exceed by 3 bits, so shiftAmt = 3.
+
+  -- and convert to target precision:
+  --                  ↓ guard
+  --  0 . 0 0 0 1 a b c d e f g h * 2^exp + 2^shiftAmt | to make 'exp + shiftAmt >= minNormalExp'.
+  --  ==============↑ (6 bits of precision)
+  -- (sigWidth - 1) - (targetSignificandWidth - 1) -
+  -- let targetSigWithHidden : BitVec (targetSignificandWidth + 1) :=
+  --   sigWithHidden.extractMsb' 0 (targetSignificandWidth + 1)
+  -- to grab the bit *after* w bits, it's the bit x[w].
+  -- we want the bit *after* targetSignificandWidth + 1, i.e., bit at index targetSignificandWidth + 1.
+  let guardBitIndexFromLsb : BitVec sigWidth :=
+    BitVec.ofNat sigWidth ((sigWidth - 1) - (targetSignificandWidth + 1))
+  -- | See that when we call 'shiftAmtPositive.zeroExtend sigWidth', there is
+  -- a potential that shiftAmtPositive is wider than sigWidth.
+  -- However, when we compute early underflow,
+  let guardBitIndexFromLsbAdjusted : BitVec sigWidth :=
+    guardBitIndexFromLsb + shiftAmtPositive.zeroExtend sigWidth
+
+  let guardBitMask : BitVec sigWidth := BitVec.oneHotBV guardBitIndexFromLsbAdjusted
+  let guardBit : Bool := (sigWithHidden &&& guardBitMask) ≠ 0#sigWidth
+  let stickyBitsMask : BitVec sigWidth := (BitVec.orderEncode guardBitIndexFromLsbAdjusted)
+  let stickyBits : BitVec sigWidth := (sigWithHidden &&& stickyBitsMask)
+  let stickyBit : Bool := stickyBits ≠ 0#sigWidth
+
+  let sigwithHiddenCleared : BitVec sigWidth :=
+    sigWithHidden &&& (~~~(guardBitMask ||| stickyBitsMask))
+
+  let lsbMask : BitVec sigWidth :=
+     BitVec.oneHotBV (guardBitIndexFromLsbAdjusted + 1#sigWidth)
+
+  let isEven : Bool := sigWithHidden &&& lsbMask = 0#sigWidth
+  let shouldRoundUp := roundingDecision
+    (mode := mode)
+    (sign := inUf.sign)
+    (significandEven := isEven)
+    (guardBit := guardBit)
+    (stickyBit := stickyBit)
+    (exact := false)
+
+  let sigDidOverflow_RoundedTargetSigWithHidden : BitVec (sigWidth + 1) :=
+    if shouldRoundUp then
+      sigwithHiddenCleared.zeroExtend (sigWidth + 1) + lsbMask.zeroExtend (sigWidth + 1)
+    else
+      sigwithHiddenCleared.zeroExtend (sigWidth + 1)
+
+  let sigDidOverflow : Bool :=
+    sigDidOverflow_RoundedTargetSigWithHidden.msb
+
+  let roundedTargetSigWithHidden : BitVec sigWidth :=
+    sigDidOverflow_RoundedTargetSigWithHidden.setWidth sigWidth
+
+  -- | This makes bollu sad, because this is the sensible way to write this.
+  -- let (roundedTargetSigWithHidden, sigDidOverflow) : BitVec sigWidth × Bool :=
+  --   if shouldRoundUp then
+  --     addWithFlags
+  --       (a := sigwithHiddenCleared)
+  --       (b := lsbMask)
+  --   else
+  --     (sigwithHiddenCleared, false)
+
+  let roundedTargetSigWithHiddenOverflowAdjusted : BitVec sigWidth :=
+    if sigDidOverflow then
+      lsbMask
+    else
+      roundedTargetSigWithHidden
+
+  let roundedExpDidOverflow_roundedExp : BitVec (expWidth + 1) :=
+    if sigDidOverflow then
+      exp.zeroExtend (expWidth + 1) + 1#(expWidth + 1)
+    else
+      exp.zeroExtend (expWidth + 1)
+
+  let roundedExpDidOverflow : Bool :=
+    roundedExpDidOverflow_roundedExp.msb
+  let roundedExp : BitVec expWidth :=
+    roundedExpDidOverflow_roundedExp.setWidth expWidth
+
+  -- I find this width stuff confusing, which width should we use?
+  -- have : expWidth ≥ exponentWidth targetExponentWidth targetSignificandWidth := by grind
+  let maxNormalExpBV : BitVec (expWidth) :=
+    BitVec.ofInt (expWidth)
+      (maxNormalExp targetExponentWidth)
+  let lateOverflow : Bool :=
+    maxNormalExpBV.slt roundedExp
+
+  let subnormalExpBV : BitVec (expWidth) :=
+    BitVec.ofInt (expWidth)
+      (subnormalExp targetExponentWidth)
+  let lateUnderflow : Bool :=
+    roundedExp.slt subnormalExpBV
+
+  let underflow : Bool := lateUnderflow || earlyUnderflow
+
+  let overflow : Bool := lateOverflow || earlyOverflow || roundedExpDidOverflow
+
+  let finalExp := roundedExp.truncate (exponentWidth targetExponentWidth targetSignificandWidth)
+  let finalSigTruncated := roundedTargetSigWithHiddenOverflowAdjusted.extractMsb' 0 (targetSignificandWidth + 1)
+  let finalNumber : UnpackedFloat (exponentWidth targetExponentWidth targetSignificandWidth) (targetSignificandWidth + 1) :=
+    { sign := inUf.sign,
+      ex := finalExp,
+      sig := finalSigTruncated
+    }
+
+  let result := rounderSpecialCases
+    (roundingMode := mode)
+    finalNumber overflow underflow inUf.isZero
+  result
+
+@[simp]
+theorem Prod.ite_fst {α β : Type} (cond : Bool) (p q : α × β) :
+    (ite cond p q).fst =
+  ite cond p.fst q.fst := by grind
+
+theorem debugRound_eq_round {expWidth sigWidth : Nat} {targetExponentWidth targetSignificandWidth : Nat}
+  (inUf : UnpackedFloat expWidth sigWidth)
+  (mode : RoundingMode) :
+  (UnpackedFloat.debugRound (targetExponentWidth := targetExponentWidth) (targetSignificandWidth := targetSignificandWidth)
+    inUf mode).1 =
+  UnpackedFloat.round (targetExponentWidth := targetExponentWidth) (targetSignificandWidth := targetSignificandWidth)
+    inUf mode := rfl
+
+def UnpackedFloat.toString {expWidth sigWidth : Nat} (uf : UnpackedFloat expWidth sigWidth) : String :=
+  s!"{if uf.sign then "-" else "+"} {uf.sig.toNat} * 2^-({sigWidth - 1}) * 2^{uf.ex.toInt}"
+
+
+def checkRoundCorrect (EUnpacked SUnpacked : Nat) (EOut SOut : Nat) : IO Bool := do
+  let mut outError : String := ""
+  let mut nsucceeded : Nat := 0
+  let mut nfailed : Nat := 0
+
+  for originalPacked in mkPackedFloats EUnpacked SUnpacked do
+    let originalEUnpacked := originalPacked.unpack
+    if ! originalEUnpacked.isNumber then continue
+
+    let originalUnpacked := originalEUnpacked.num
+    let originalNormalized := originalUnpacked.normalize
+    let (outputRoundedEUnpacked, log) :=
+      UnpackedFloat.debugRound (targetExponentWidth := EOut) (targetSignificandWidth := SOut)
+        originalNormalized RoundingMode.RNE
+    let outputRoundedPacked := outputRoundedEUnpacked.pack
+    let expectedEUnpacked :=
+      getClosestRNEResult (targetExponentWidth := EOut) (targetSignificandWidth := SOut)
+        originalUnpacked
+    let expectedPacked := expectedEUnpacked.normalize.pack
+    if outputRoundedPacked.equal_denotation expectedPacked then
+      IO.println s!"Succeeded ✅ | original {repr originalEUnpacked}"
+      nsucceeded := nsucceeded + 1
+    else
+      let err : String := ""
+      let err := err ++ s!"\nFailed ❌ | original {repr originalEUnpacked}"
+      let err := err ++ s!"\n  original (Q) {repr originalPacked.toRat?}"
+      let err := err ++ s!"\n  --"
+      let err := err ++ s!"\n  output rounded (eunpacked) {repr outputRoundedEUnpacked}"
+      let err := err ++ s!"\n  output rounded (Q) {repr outputRoundedEUnpacked.toRat?}"
+      let err := err ++ s!"\n  --"
+      let err := err ++ s!"\n  expected (Q) {repr expectedPacked.toRat?}"
+      let err := err ++ s!"\n  expected (eunpacked) {repr expectedEUnpacked}"
+      -- let err := err ++ s!"\n  expected packed {repr expectedPacked}"
+      let err := err ++ s!"\n\n{log}"
+      IO.println err
+      outError := err
+      nfailed := nfailed + 1
+  if nfailed = 0 then
+    IO.println "All succeeded ✅"
+  else
+    -- | this is fixed point, with two digits of precision.
+    let fracSuccess : Float := (nsucceeded.toFloat * 100.0) / ((nsucceeded + nfailed).toFloat)
+    throw (IO.Error.userError s!"({nsucceeded} succeeded / {nsucceeded + nfailed} total) ({fracSuccess}% succeeded) ❌\n{outError}")
+  return nfailed = 0
+/--
+error: (716 succeeded / 992 total) (72.177419% succeeded) ❌
+
+Failed ❌ | original { state := num, num := { sign := false, ex := 0x0f#6, sig := 0x1b#5 } }
+  original (Q) some 55296
+  --
+  output rounded (eunpacked) { state := num, num := { sign := false, ex := 0x0f#5, sig := 0x3#2 } }
+  output rounded (Q) some 49152
+  --
+  expected (Q) none
+  expected (eunpacked) { state := ∞, num := { sign := false, ex := 0x00#5, sig := 0x0#2 } }
+
+
+--- rounding: { sign := false, ex := 0x0f#6, sig := 0x1b#5 } ---
+  val (Q): 55296 = sig(0b11011=nat:27)) * 2 ** exp:([0b001111=int:15] - (4))
+exp: 0b001111 = int:15
+targetMinNormalExp: 0b110010 = int:-14
+maxNormalExp: 15
+earlyOverflow: false
+minSubnormalExp: -16
+earlyUnderflow: false
+expGeMin: 0b001111 = int:15
+shiftAmtPositive: 0b000000 = int:0 = nat:0
+sigWithHidden: 0b11011 = nat:27
+guardBitIndexFromLsb: (sigWidth(5) - 1)  - (targetSignificandWidth(1) + 1) = 2
+guardBitIndexFromLsb: 0b00010 = nat:2
+guardBitIndexFromLsbAdjusted: 0b00010 = nat:2
+guardBitMask: 0b00100
+guardBit: false = 0b11011 &&& 0b00100
+stickyBitsMask: 0b00011
+stickyBits: 0b00011
+stickyBit: true = 0b11011 &&& 0b00011
+sigwithHiddenCleared: 0b11000 = 0b11011 &&& ~(0b00100 ||| 0b00011)
+lsbMask: 0b01000
+isEven: false = 0b11011 &&& 0b01000
+shouldRoundUp: false
+roundedTargetSigWithHidden = sigwithHiddenCleared(0b11000)
+roundedTargetSigWithHidden: 0b11000 = nat:24
+sigDidOverflow: false
+roundedTargetSigWithHiddenOverflowAdjusted: 0b11000 = nat:24
+roundedExp: 0b001111 = int:15
+roundedExpDidOverflow: false
+late overflow: false = roundedExp(0b001111=int:15) > maxNormalExpBV(0b001111=int:15)
+late underflow: false = maxNormalExpBV(0b001111=int:15) < roundedExp(0b001111=int:15)
+underflow: false = lateUnderflow(false) || earlyUnderflow(false)
+overflow: false = lateOverflow(false) || earlyOverflow(false)
+-/
+#guard_msgs(error) in #eval checkRoundCorrect 5 4 5 1
+
+def checkNormalizeIdem (E S : Nat) : IO Bool := do
+  let mut allSucceeded := true
+  for originalPacked in mkPackedFloats E S do
+    if ! originalPacked.isNorm then continue -- we only need to think about the normal case for now.
+    let originalEUnpacked := originalPacked.unpack
+    -- if ! originalEUnpacked.isNumber then continue
+    let originalUnpacked := originalEUnpacked.num
+    let originalUnpackedNormalized := originalUnpacked.normalize
+
+    let outputUnpacked := EUnpackedFloat.mkNumber originalUnpackedNormalized
+    let outputPacked := outputUnpacked.pack
+    if ! originalPacked.equal_denotation outputPacked then
+      IO.println s!"Failed ❌ | original {repr originalPacked.toRat?} → output {repr outputPacked.toRat?}"
+      allSucceeded := false
+  if allSucceeded then
+    IO.println "All succeeded ✅"
+  else
+    throw (IO.Error.userError "Some failed ❌")
+  return allSucceeded
+
+/--
+info: All succeeded ✅
+---
+info: true
+-/
+#guard_msgs in #eval checkNormalizeIdem 3 5
+theorem foo (x y : BitVec 5) (b : Bool) :
+  let z := if b then x else y
+  let w := if ! b then y else x
+  z = w := by bv_decide
